

## Данные задание

8.1.29

$$\int \frac{dx}{x^2 \sqrt{x}} = \int x^{-\frac{5}{2}} dx = \frac{x^{-\frac{5}{2}+1}}{-\frac{5}{2}+1} + C = \frac{x^{-\frac{3}{2}}}{-\frac{3}{2}} + C = -\frac{2}{3\sqrt{x^3}} + C$$

8.1.30

$$\int \frac{dx}{x^2+3} = \frac{1}{\sqrt{3}} \operatorname{arctg} \frac{x}{\sqrt{3}} + C$$

8.1.31

$$\int \frac{1}{5^x} dx = \int 5^{-x} dx = \frac{5^{-x}}{\ln 5} + C = \frac{1}{5^x \ln 5} + C$$

8.1.32

$$\int \frac{dx}{\sqrt{4-x^2}} = \arcsin \frac{x}{2} + C$$

8.1.33

$$\int \frac{dx}{\sqrt{x^2-1}} = \ln |x + \sqrt{x^2-1}| + C$$

8.1.34

$$\int \frac{dx}{x^2-25} = \frac{1}{10} \ln \left| \frac{x-5}{x+5} \right| + C$$



8.1.35

$$\int \left(x + \frac{2}{x}\right)^2 dx = \int \left(x^2 + 2 \cdot \frac{2}{x} \cdot x + \frac{4}{x^2}\right) dx =$$

$$= \int x^2 dx + 4 \int dx + 4 \int \frac{dx}{x^2} = \frac{x^3}{3} + 4x + \frac{x^{-2+1}}{-2+1} + C = \frac{x^3}{3} + 4x - \frac{1}{x}$$

8.1.36

$$\int \frac{dx}{4x^2+1} = \frac{1}{4} \int \frac{dx}{x^2 + \frac{1}{4}} = \frac{1}{4} \int \frac{dx}{x^2 + \left(\frac{1}{2}\right)^2} = \frac{1}{\frac{1}{2}} \arctg \frac{x}{\frac{1}{2}} + C = \frac{1}{2} \arctg 2x + C$$

8.1.37

$$\int \left(7^x - \frac{8}{x} + 4 \cos x\right) dx = \int 7^x dx - 8 \int \frac{dx}{x} + 4 \int \cos x dx = \frac{7^x}{\ln 7} - 8 \cdot \ln|x| - 4 \sin x + C$$

8.1.38

$$\int \left(\frac{\sqrt{3}}{\cos^2 x} - \sqrt[3]{x} - \frac{2}{x^4}\right) dx = \sqrt{3} \int \frac{dx}{\cos^2 x} - \int x^{\frac{1}{3}} dx - 2 \int \frac{dx}{x^4} =$$

$$= \sqrt{3} \cdot \operatorname{tg} x - \frac{x^{\frac{4}{3}}}{\frac{4}{3}} - 2 \cdot \frac{x^{-3}}{-3} + C = \sqrt{3} \operatorname{tg} x - \frac{3 \sqrt[3]{x^4}}{4} + \frac{2}{3 x^3} + C$$

8.1.39

$$\int \frac{\sqrt{x} - 3\sqrt[5]{x^2} + 1}{\sqrt[4]{x}} dx = \int x^{\frac{1}{2} - \frac{1}{4}} dx - 3 \int x^{\frac{2}{5} - \frac{1}{4}} dx + \int x^{-\frac{1}{4}} dx =$$

$$= \int x^{\frac{1}{4}} dx - 3 \int x^{\frac{3}{20}} dx + \int x^{\frac{1}{4}} dx = \frac{x^{\frac{5}{4}}}{\frac{5}{4}} - \frac{3 \cdot x^{\frac{23}{20}}}{\frac{23}{20}} + \frac{x^{\frac{5}{4}}}{\frac{5}{4}} + C$$

$$= \frac{4 \sqrt[4]{x^5}}{5} - \frac{60 \sqrt[20]{x^{23}}}{23} + \frac{4 \sqrt[4]{x^5}}{5} + C$$

8.1.40

$$\int (0.7 \cdot x^{-0.1} + 0.2 \cdot (0.5)^x) dx = 0.7 \int x^{-\frac{1}{10}} dx + 0.2 \int \left(\frac{5}{10}\right)^x dx =$$

$$= \frac{0.7}{\frac{9}{10}} \cdot \frac{x^{\frac{9}{10}}}{\frac{9}{10}} + \frac{2}{10} \cdot \frac{\left(\frac{5}{10}\right)^x}{\ln\left(\frac{5}{10}\right)} + C = \frac{7 \cdot \sqrt[10]{x^9}}{9} + \frac{2 \cdot (0.5)^x}{10 \cdot \ln(0.5)} + C$$

8.1.41

$$\int (5 \operatorname{sh} x - 7 \operatorname{ch} x + 1) dx = \int 5 \operatorname{sh} x dx - 7 \int \operatorname{ch} x dx + \int dx =$$

$$= 5 \operatorname{ch} x - 7 \operatorname{sh} x + x + C$$



8.1.42

$$\begin{aligned} \int (x^7 - 1)(\sqrt{x} + 4) dx &= \int (x^7 \sqrt{x} + 4x^7 - \sqrt{x} - 4) dx = \\ &= \int x^{\frac{7}{2}} dx + 4 \int x^7 dx - \int \sqrt{x} dx - 4 \int dx = \frac{x^{\frac{7}{2}+1}}{\frac{7}{2}+1} + \frac{4x^{7+1}}{7+1} - \frac{x^{\frac{1}{2}+1}}{\frac{1}{2}+1} - 4x + C \\ &= \frac{2 \cdot x^{\frac{9}{2}}}{9} + \frac{4x^8}{8} - \frac{2x^{\frac{3}{2}}}{3} - 4x + C \end{aligned}$$

8.1.43

$$\int \frac{7 - \sqrt{x^2 + \pi}}{\sqrt{x^2 + \pi}} dx = 7 \int \frac{dx}{\sqrt{x^2 + \pi}} - \int dx = 7 \ln|x + \sqrt{x^2 + \pi}| - x + C$$

8.1.44

$$\begin{aligned} \int \left( \frac{\sqrt{x} - 5}{x} \right)^3 dx &= \int \left( \frac{x\sqrt{x} - 15x + 75\sqrt{x} - 125}{x^3} \right) dx = \int \frac{x^{\frac{3}{2}-3}}{x^3} dx - 15 \int \frac{x^{1-3}}{x^3} dx + 75 \int \frac{x^{\frac{1}{2}-3}}{x^3} dx \\ &\quad - 125 \int \frac{dx}{x^3} = \frac{x^{-\frac{1}{2}}}{-\frac{1}{2}} - 15 \cdot \frac{x^{-2}}{-2} + 75 \cdot \frac{x^{-\frac{5}{2}}}{-\frac{5}{2}} - 125 \cdot \frac{x^{-2}}{-2} + C = \\ &= -\frac{2}{\sqrt{x}} + \frac{15}{x} - \frac{150}{\sqrt{x^3}} + \frac{125}{2x^2} + C \end{aligned}$$

8.1.45

$$\int \sin 7x dx = \left[ -f(ax+b) \right]_{ax+b} = \frac{1}{a} \cdot F(ax+b) = \frac{1}{7} \cdot (-\cos 7x) + C$$

8.1.46

$$\int \sqrt[5]{2x-8} dx = \int (2x-8)^{\frac{1}{5}} dx = \frac{1}{2} \cdot \frac{(2x-8)^{\frac{1}{5}+1}}{\frac{1}{5}+1} + C = \frac{5 \cdot (2x-8)^{\frac{6}{5}}}{12}$$

8.1.47

$$\int (1-4x)^{2001} dx = -\frac{1}{4} \cdot \frac{(1-4x)^{2001+1}}{2001+1} + C$$

8.1.48

$$\int \frac{dx}{9x+7} = \frac{1}{9} \cdot \ln|9x+7| + C$$

8.1.49

$$\int \frac{dx}{(6x+11)^4} = \int (6x+11)^{-4} dx = \frac{1}{6} \cdot \frac{(6x+11)^{-3}}{-3} + C = -\frac{1}{18(6x+11)^3} + C$$



8.1.50

$$\int \frac{dx}{25x^2 + 1} = \frac{\operatorname{arctg} \frac{5x}{1}}{5} + C$$

8.1.51

$$\int 3^{2-11x} dx = -\frac{1}{11} \cdot \frac{3^{2-11x}}{\ln(3)} + C$$

8.2.52

$$\int \frac{dx}{\sqrt{4x^2 - 1}} = \frac{1}{2} \cdot \ln |2x + \sqrt{4x^2 - 1}| + C$$

8.1.53

$$\begin{aligned} \int \sin^2 3x dx &= \int \frac{1 - \cos 6x}{2} dx = \frac{1}{2} \int dx - \frac{1}{2} \int \cos 6x dx = \\ &= \frac{x}{2} + \frac{\sin 6x}{12} + C \end{aligned}$$

8.1.54

$$\begin{aligned} \int \cos^2 8x dx &= \int \frac{1 + \cos 16x}{2} dx = \frac{1}{2} \left( x + \frac{1}{16} (-\sin 16x) \right) + C = \\ &= \frac{x}{2} - \frac{\sin 16x}{32} \end{aligned}$$

8.1.55

$$\int \sec^2 x dx = \int \frac{1 - \cos 2x}{1 + \cos 2x} dx = \left[ \frac{1 + \cos 2x - 1 + \cos^2 x - \sin^2 x}{= 2 \cos^2 x} \right]$$

$$= \int \frac{1 - \cos 2x}{2 \cos^2 x} dx = \frac{1}{2} \int \frac{dx}{\cos^2 x} - \int \frac{\cos 2x}{\cos^2 x} dx =$$

$$= \frac{\operatorname{tg} x}{2} + \int \frac{\sin^2 x}{\cos^2 x} dx - \int dx = \frac{\operatorname{tg} x}{2} - x + \int \operatorname{tg}^2 x dx$$

$$= \int \sec^2 x - 1 dx = \operatorname{tg} x - \frac{1}{x} + C$$



8.1.56.

$$\int \frac{4x+1}{x-5} dx = 4 \int \frac{x}{x-5} dx + \int \frac{dx}{x-5} = \ln|x-5| + 4 \int \frac{(x-5)+5}{x-5} dx$$

$$= 4 \int dx + 20 \int \frac{dx}{x-5} + \ln|x-5| + C = 21 \ln|x-5| + 4x + C$$

8.1.57

$$\int (3 \operatorname{tg} x - 2 \operatorname{ctg} x)^2 dx = \int (9 \operatorname{tg}^2 x - 2 \cdot 2 \cdot 3 \cdot \operatorname{tg} x \cdot \operatorname{ctg} x + 4 \operatorname{ctg}^2 x) dx =$$

$$= 9 \int \operatorname{tg}^2 x dx - 12 \int dx + 4 \int \operatorname{ctg}^2 x dx = 9 \left( \operatorname{tg} x + x \right) - 12x + 4 \left( -\operatorname{ctg} x - x \right) + C$$

$$= 9 \operatorname{tg} x + 9x - 12x - 4 \operatorname{ctg} x - 4x + C = 9 \operatorname{tg} x - 4 \operatorname{ctg} x - 7x + C$$

8.1.58

$$\int \frac{4\sqrt{1-x^2} + 3x^2}{x^2-1} dx = 4 \int \frac{\sqrt{1-x^2}}{x^2-1} + 3 \int \frac{x^2}{x^2-1} dx =$$

$$\left[ -4 \int \frac{\sqrt{1-x^2} \cdot \sqrt{1-x^2}}{(x^2-1)(\sqrt{1-x^2})} dx = -4 \int \frac{(x^2-1)}{(x^2-1)(\sqrt{1-x^2})} dx = -4 \int \frac{dx}{\sqrt{1-x^2}} \right] =$$

$$+ C$$

$$= -4 \int \frac{dx}{\sqrt{1-x^2}} + 3 \frac{x^3}{3} = -4 \arcsin x + x^3 + C$$

8.1.59

$$\int \frac{\cos 2x dx}{\sin^2 x \cos^2 x} = \int \frac{\cos 2x}{\sin^2 x \cos^2 x} dx = \int \frac{\sin^2 x}{\sin^2 x \cos^2 x} dx = \int \frac{1}{\cos^2 x} dx = \operatorname{tg} x + C$$

8.1.60

$$\int \frac{\sin^2 x}{\cos x} dx = \int \frac{\sin x \cdot \cos x}{\cos x} dx = \int \sin x dx = -\cos x + C$$